Hash table proof uses Gospel definitions

zoo/hashtbl/lib/hashtbl.mli
@@ -5,13 +5,27 @@ type ('k, 'v) t
 
 val create : int -> ('k, 'v) t
 (*@ h = create n
+    requires n > 0
     ensures h = ∅ *)
-
-val population : ('k, 'v) t -> int
-(*@ n = population h
-    ensures n = Fin_maps.population h *)
 
 val add : ('k, 'v) t -> 'k -> 'v -> unit
 (*@ add h k v
     modifies h
     ensures h = add k (Sequence.cons v (old (h[k]))) (old h) *)
+
+(*@ function cardinality (m : ('k, 'v sequence) fin_map) : integer =
+      fold (λ k s acc -> acc + Sequence.length s) 0 m *)
+
+val population : ('k, 'v) t -> int
+(*@ n = population h
+    ensures n = cardinality h *)
+
+(* @ predicate permitted *)
+(*     (m : fin_map val (val sequence)) (h : ('k * 'v) sequence) *)
+
+(* val iter :  *)
+(* (\*@ iter_rev h f m, *)
+(*     ITER *)
+(*     ~permitted:(permitted m) *)
+(*     ~complete:(complete m) *)
+(*     ~step:(fun x => let (k, v) = x in f k v) *\) *)
